# Readme

**This project is the code for the T4 of the following question.**

## Question

Consider the following grammar:
$$
exp→exp+factor\ |\ factor
\newline
factor→{\bf (}exp{\bf )}\ |\ {\bf number}
$$

1.  Eliminate the left recursion using BNF;
2. Design an L-SDD to compute the value of the expression generated by the grammar of (1);
3. Convert the SDD of (2) to SDT;
4. Implement the SDT of (3) as a recursive-descent parser.

## T1

$$
exp→factor\ exp'
\newline
exp'→+factor\ exp'\ |\ \epsilon
\newline
factor→{\bf (}exp{\bf )}\ |\ {\bf number}
$$

## T2

|          PRODUCTION          |                        SEMANTIC RULES                        |
| :--------------------------: | :----------------------------------------------------------: |
|      $exp→factor\ exp'$      |        $exp'.inh=factor.syn$<br />$exp.syn=exp'.syn$         |
| $exp'_{1}→+factor\ exp'_{2}$ | $exp'_{2}.inh=exp'_{1}.inh+factor.syn$<br />$exp'_{1}.syn=exp'_{2}.syn$ |
|       $exp'→\epsilon$        |                     $exp'.syn=exp'.inh$                      |
|  $factor→{\bf (}exp{\bf )}$  |                     $factor.syn=exp.syn$                     |
|    $factor→{\bf number}$     |               $factor.syn={\bf number}.lexval$               |

## T3

|          PRODUCTION          |                        SEMANTIC RULES                        |                           ACTIONS                            |
| :--------------------------: | :----------------------------------------------------------: | :----------------------------------------------------------: |
|      $exp→factor\ exp'$      |        $exp'.inh=factor.syn$<br />$exp.syn=exp'.syn$         | $exp→factor\{exp'.inh=factor.syn\}\newline exp'\{exp.syn=exp'.syn\}$ |
| $exp'_{1}→+factor\ exp'_{2}$ | $exp'_{2}.inh=exp'_{1}.inh+factor.syn$<br />$exp'_{1}.syn=exp'_{2}.syn$ | $exp'_{1}→+factor\{exp'_{2}.inh=exp'_{1}.inh+factor.syn\}\newline exp'_{2}\{exp'_{1}.syn=exp'_{2}.syn\}$ |
|       $exp'→\epsilon$        |                     $exp'.syn=exp'.inh$                      |             $exp'→\epsilon\{exp'.syn=exp'.inh\}$             |
|  $factor→{\bf (}exp{\bf )}$  |                     $factor.syn=exp.syn$                     |       $factor→{\bf (}exp{\bf )}\{factor.syn=exp.syn\}$       |
|    $factor→{\bf number}$     |               $factor.syn={\bf number}.lexval$               |   $factor→{\bf number}\{factor.syn={\bf number}.lexval\}$    |

## T4

- Code: Please refer to the source code.
